Modified Gmap using map interface

inductive_proof/Grow-only_map/App.fst
@@ -1,47 +1,22 @@
 module App
 
-module L = FStar.List.Tot
+module M = Map_extended
+module S = FStar.Set
 
 #set-options "--query_stats"
-let rec unique_s (l:list nat) =
-  match l with
-  |[] -> true
-  |id::xs -> not (L.mem id xs) && unique_s xs
-
-type gset_st = l:list nat{unique_s l}
-
-let rec mem_k (k:nat) (l:list (nat * gset_st)) : (b:bool{(exists e. L.mem e l /\ fst e = k) /\ (exists s. L.mem (k,s) l) <==> b = true}) =
-  match l with
-  |[] -> false
-  |(k1,s)::xs -> k1 = k || mem_k k xs
-
-let rec unique_k (l:list (nat * gset_st)) =
-  match l with
-  |[] -> true
-  |(x,s)::xs -> not (mem_k x xs) && unique_k xs
 
 // the concrete state type
 // It is a list of unique elements
-type concrete_st = l:list (nat * gset_st){unique_k l}
-
-let rec mem_kv (k v:nat) (l:concrete_st) 
-  : (b:bool{b = true <==> ((exists e. L.mem e l /\ fst e = k /\ L.mem v (snd e)) /\ mem_k k l /\
-                         (exists s. L.mem (k,s) l))}) =
-  match l with
-  |[] -> false
-  |x::xs -> (k = fst x && L.mem v (snd x)) || mem_kv k v xs
-
-let rec get_set (k:nat) (st:concrete_st{mem_k k st}) 
-    : (r:gset_st{L.mem (k,r) st /\ (forall e. L.mem e r <==> mem_kv k e st)}) =
-  match st with
-  |[] -> []
-  |(x,s)::xs -> if x = k then s else get_set k xs
+type concrete_st = M.t nat (S.set nat)
 
 //initial state
-let init_st = []
+let init_st = M.const S.empty
+
+let sel (s:concrete_st) k = if M.contains s k then M.sel s k else S.empty
 
 let eq (a b:concrete_st) =
-  (forall k v. mem_kv k v a <==> mem_kv k v b)
+  (forall id. M.contains a id = M.contains b id /\
+         S.equal (sel a id) (sel b id))
 
 let symmetric (a b:concrete_st) 
   : Lemma (requires eq a b)
@@ -52,7 +27,7 @@ let transitive (a b c:concrete_st)
           (ensures eq a c) = ()
 
 let eq_is_equiv (a b:concrete_st)
-  : Lemma (requires a = b)
+  : Lemma (requires a == b)
           (ensures eq a b) = ()
           
 // operation type
@@ -63,212 +38,162 @@ let key (op:op_t) = fst (snd op)
 
 let value (op:op_t) = snd (snd op)
 
-#push-options "--z3rlimit 100"
-let rec add_v (k v:nat) (s:concrete_st)
-  : Pure concrete_st 
-    (requires mem_k k s)
-    (ensures (fun r -> (forall k1. mem_k k1 r <==> mem_k k1 s) /\
-                    (forall e. L.mem e r /\ fst e <> k <==> L.mem e s /\ fst e <> k) /\
-                    (forall (e1 e2:nat * gset_st). L.mem e1 s /\ L.mem e2 r /\ fst e1 = k /\ fst e2 = k ==> 
-                               (forall e3. L.mem e3 (snd e1) \/ e3 = v <==> L.mem e3 (snd e2))) /\
-                    (forall k1 v1. mem_kv k1 v1 r <==> mem_kv k1 v1 s \/ (k1 = k /\ v1 = v)))) =
-  match s with
-  |x::xs -> if k = fst x && L.mem v (snd x) then s
-             else if k = fst x then ((k, (v::(snd x)))::xs)
-               else (x::add_v k v xs)
-
-let do (s:concrete_st) (op:op_t) 
-  : (r:concrete_st{(forall k. mem_k k r <==> mem_k k s \/ k = key op) /\
-                   (forall k v. mem_kv k v r <==> mem_kv k v s \/ (k = key op /\ v = value op)) /\
-                   (forall e. L.mem e r /\ fst e <> key op <==> L.mem e s /\ fst e <> key op)}) = 
-  match s with
-  |[] -> [key op, [value op]]
-  |x::xs -> if mem_k (key op) s then add_v (key op) (value op) s 
-             else  ((key op, [value op])::s)
-
-let do_prop (s:concrete_st) (op:op_t) 
-  : Lemma (ensures (forall k v. mem_kv k v (do s op) <==> mem_kv k v s \/ (k = key op /\ v = value op))) = ()
+let do (s:concrete_st) (op:op_t) =
+  let (ts,(k,v)) = op in
+  M.upd s k (S.union (S.singleton v) (sel s k))
 
 let lem_do (a b:concrete_st) (op:op_t)
    : Lemma (requires eq a b)
-           (ensures eq (do a op) (do b op)) =
-   do_prop a op;
-   do_prop b op
+           (ensures eq (do a op) (do b op)) = ()
 
 //conflict resolution
 let resolve_conflict (x:op_t) (y:op_t{fst x <> fst y}) : resolve_conflict_res = First_then_second
-
-// concrete merge operation
-let rec concrete_merge_g (lca s1 s2:gset_st)
-  : Pure gset_st (requires true)
-                     (ensures (fun r -> (forall e. L.mem e r <==> L.mem e lca \/ L.mem e s1 \/ L.mem e s2)))
-                     (decreases %[lca;s1;s2]) =
-  match lca, s1, s2 with
-  |[],[],[] -> []
-  |x::xs,_,_ -> if L.mem x s1 || L.mem x s2 then concrete_merge_g xs s1 s2 else x::concrete_merge_g xs s1 s2
-  |[],x::xs,_ -> if L.mem x s2 then concrete_merge_g [] xs s2 else x::(concrete_merge_g [] xs s2)
-  |[],[],x::xs -> x::concrete_merge_g [] [] xs
-
-let rec rem_k (k:nat) (l:concrete_st)
-    : Tot (r:concrete_st{(forall e. L.mem e r <==> L.mem e l /\ fst e <> k) /\
-                         (forall k1 v1. mem_kv k1 v1 r <==> mem_kv k1 v1 l /\ k1 <> k)}) = 
-  match l with
-  |[] -> []
-  |(x,s)::xs -> if k = x then xs else (x,s)::rem_k k xs
-
-#push-options "--z3rlimit 500 --fuel 2 --ifuel 2"
-let rec concrete_merge1 (lca:concrete_st) (s1:concrete_st) (s2:concrete_st)
-  : Pure concrete_st (requires true)
-                     (ensures (fun r -> (forall k. mem_k k r <==> mem_k k lca \/ mem_k k s1 \/ mem_k k s2) /\
-                                     (forall k v. mem_kv k v r <==> mem_kv k v lca \/ mem_kv k v s1 \/ mem_kv k v s2)))
-                     (decreases %[lca;s1; s2]) =
-  match lca, s1, s2 with
-  |[],[],[] -> []
-  |(k,s)::xs,_,_ -> if mem_k k s1 && mem_k k s2 then
-                    (k, concrete_merge_g s (get_set k s1) (get_set k s2))::concrete_merge1 xs (rem_k k s1) (rem_k k s2)
-                  else if mem_k k s1 then
-                    (k, concrete_merge_g s (get_set k s1) [])::concrete_merge1 xs (rem_k k s1) s2
-                  else if mem_k k s2 then
-                    (k, concrete_merge_g s [] (get_set k s2))::concrete_merge1 xs s1 (rem_k k s2)
-                  else (k,s)::concrete_merge1 xs s1 s2
-  |[],(k,s)::xs,_ -> if mem_k k s2 then (k, concrete_merge_g [] s (get_set k s2))::concrete_merge1 [] xs (rem_k k s2)
-                   else (k,s)::concrete_merge1 [] xs s2
-  |[],[],_ -> s2
-#pop-options
 
 // concrete merge operation
 let concrete_merge (lca s1 s2:concrete_st) 
   : Pure concrete_st
          (requires (exists l1 l2. apply_log lca l1 == s1 /\ apply_log lca l2 == s2))
          (ensures (fun _ -> True)) =
-  concrete_merge1 lca s1 s2
+  let keys = S.union (M.domain lca) (S.union (M.domain s1) (M.domain s2)) in
+  let u:concrete_st = M.const_on keys S.empty in
+  M.iter_upd (fun k v -> S.union (sel lca k) (S.union (sel s1 k) (sel s2 k))) u
 
 let merge_is_comm (lca s1 s2:st)
   : Lemma (requires consistent_branches lca s1 s2)
           (ensures (eq (concrete_merge (v_of lca) (v_of s1) (v_of s2)) 
                        (concrete_merge (v_of lca) (v_of s2) (v_of s1)))) = ()
-                       
-let linearizable_s1_0''_base_base (lca s1 s2':st) (last2:op_t)
-  : Lemma (requires consistent_branches lca s1 (do_st s2' last2) /\
-                    ops_of s1 = ops_of lca /\ ops_of s2' = ops_of lca /\
-                    length (ops_of lca) = 0)
-        
-          (ensures eq (do (v_of s2') last2) (concrete_merge (v_of lca) (v_of s1) (do (v_of s2') last2))) = ()
 
-let linearizable_s1_0''_base_ind (lca s1 s2':st) (last2:op_t)
-  : Lemma (requires consistent_branches lca s1 (do_st s2' last2) /\
-                    ops_of s1 = ops_of lca /\ ops_of s2' = ops_of lca /\
-                    length (ops_of lca) > 0 /\
-
-                    (let l' = inverse_st lca in
-                    let s1' = inverse_st s1 in
-                    let s2'' = inverse_st s2' in
-                    consistent_branches l' s1' (do_st s2'' last2) /\
-                    ops_of s1' = ops_of l' /\ ops_of s2'' = ops_of l' /\
-                    eq (do (v_of s2'') last2) (concrete_merge (v_of l') (v_of s1') (do (v_of s2'') last2))))
-
-          (ensures eq (do (v_of s2') last2) (concrete_merge (v_of lca) (v_of s1) (do (v_of s2') last2))) = ()
-
-let linearizable_s1_0''_ind (lca s1 s2':st) (last2:op_t)
-  : Lemma (requires consistent_branches lca s1 (do_st s2' last2) /\
-                    ops_of s1 = ops_of lca /\
-                    length (ops_of s2') > length (ops_of lca) /\
-
-                    (let inv2 = inverse_st s2' in
-                    consistent_branches lca s1 (do_st inv2 last2) /\
-                    eq (do (v_of inv2) last2) (concrete_merge (v_of lca) (v_of s1) (do (v_of inv2) last2))))
-        
-          (ensures eq (do (v_of s2') last2) (concrete_merge (v_of lca) (v_of s1) (do (v_of s2') last2))) = 
-  do_prop (v_of s2') last2
-          
-let linearizable_s1_0_s2_0_base (lca s1 s2:st)
+let linearizable_s1_0_s2_0_base_direct (lca s1 s2:st)
   : Lemma (requires consistent_branches lca s1 s2 /\
-                    ops_of s1 == ops_of lca /\ ops_of s2 == ops_of lca)
-        
+                    ops_of s1 == ops_of lca /\ ops_of s2 == ops_of lca)       
           (ensures eq (v_of lca) (concrete_merge (v_of lca) (v_of s1) (v_of s2))) = ()
 
-let linearizable_gt0_base (lca s1 s2:st) (last1 last2:op_t)
-  : Lemma (requires consistent_branches lca s1 s2 /\
-                    consistent_branches lca s1 s2 /\
-                    ops_of s1 = ops_of lca /\ ops_of s2 = ops_of lca /\
-                    fst last1 <> fst last2)
-         
-          (ensures (First_then_second? (resolve_conflict last1 last2) ==>
-                      (eq (do (concrete_merge (v_of lca) (v_of s1) (do (v_of s2) last2)) last1)
-                         (concrete_merge (v_of lca) (do (v_of s1) last1) (do (v_of s2) last2))))) = 
-  do_prop (v_of s1) last1;
-  do_prop (v_of s2) last2
-
 #push-options "--z3rlimit 50"
-let linearizable_gt0_ind (lca s1 s2:st) (last1 last2:op_t)
-  : Lemma (requires consistent_branches lca (do_st s1 last1) (do_st s2 last2) /\
-                    consistent_branches lca s1 s2 /\
-                    length (ops_of s2) > length (ops_of lca) /\
-                    fst last1 <> fst last2)
-       
-          (ensures (let s2' = inverse_st s2 in
-                   ((First_then_second? (resolve_conflict last1 last2) /\
-                    consistent_branches lca s1 (do_st s2' last2) /\
-                    consistent_branches lca (do_st s1 last1) (do_st s2' last2) /\
-                    consistent_branches lca s1 (do_st s2 last2) /\
-                    eq (do (concrete_merge (v_of lca) (v_of s1) (do (v_of s2') last2)) last1)
-                       (concrete_merge (v_of lca) (do (v_of s1) last1) (do (v_of s2') last2))) ==>
-                       
-                    (eq (do (concrete_merge (v_of lca) (v_of s1) (do (v_of s2) last2)) last1)
-                        (concrete_merge (v_of lca) (do (v_of s1) last1) (do (v_of s2) last2)))))) = 
-  do_prop (v_of s1) last1;
-  do_prop (v_of s2) last2
-                       
-let linearizable_gt0_ind1 (lca s1 s2:st) (last1 last2:op_t)
-  : Lemma (requires consistent_branches lca (do_st s1 last1) (do_st s2 last2) /\
-                    consistent_branches lca s1 s2 /\
-                    length (ops_of s1) > length (ops_of lca) /\
-                    fst last1 <> fst last2)
-        
-          (ensures (let s1' = inverse_st s1 in
-                   ((ops_of s2 = ops_of lca /\
-                    First_then_second? (resolve_conflict last1 last2) /\
-                    consistent_branches lca s1' (do_st s2 last2) /\
-                    consistent_branches lca (do_st s1' last1) (do_st s2 last2) /\
-                    consistent_branches lca s1 (do_st s2 last2) /\
-                    eq (do (concrete_merge (v_of lca) (v_of s1') (do (v_of s2) last2)) last1)
-                       (concrete_merge (v_of lca) (do (v_of s1') last1) (do (v_of s2) last2))) ==>
-                       
-                    eq (do (concrete_merge (v_of lca) (v_of s1) (do (v_of s2) last2)) last1)
-                       (concrete_merge (v_of lca) (do (v_of s1) last1) (do (v_of s2) last2))))) = 
-  do_prop (v_of s1) last1;
-  do_prop (v_of s2) last2
+let linearizable_gt0_s1 (lca s1 s2:st)
+  : Lemma (requires consistent_branches_s1s2_gt0 lca s1 s2 /\
+                    consistent_branches lca (inverse_st s1) s2 /\
+                    consistent_branches lca (inverse_st s1) (inverse_st s2) /\
+                    (let _, last1 = un_snoc (ops_of s1) in
+                    let _, last2 = un_snoc (ops_of s2) in
+                    fst last1 <> fst last2 /\
+                    First_then_second? (resolve_conflict last1 last2)))
+          (ensures (let _, last1 = un_snoc (ops_of s1) in
+                   eq (do (concrete_merge (v_of lca) (v_of (inverse_st s1)) (v_of s2)) last1)
+                       (concrete_merge (v_of lca) (v_of s1) (v_of s2)))) = ()
+
+let linearizable_gt0_s2 (lca s1 s2:st)
+  : Lemma (requires consistent_branches_s1s2_gt0 lca s1 s2 /\
+                    consistent_branches lca s1 (inverse_st s2) /\
+                    consistent_branches lca (inverse_st s1) (inverse_st s2) /\
+                    (let _, last1 = un_snoc (ops_of s1) in
+                    let _, last2 = un_snoc (ops_of s2) in
+                    fst last1 <> fst last2 /\
+                    Second_then_first? (resolve_conflict last1 last2)))
+          (ensures (let _, last2 = un_snoc (ops_of s2) in                   
+                   eq (do (concrete_merge (v_of lca) (v_of s1) (v_of (inverse_st s2))) last2)
+                      (concrete_merge (v_of lca) (v_of s1) (v_of s2)))) = () 
 #pop-options
 
 ////////////////////////////////////////////////////////////////
 //// Sequential implementation //////
 
 // the concrete state 
-type concrete_st_s = concrete_st
+type concrete_st_s_direct = concrete_st
 
 // init state 
-let init_st_s = []
+let init_st_s_direct = init_st
 
 // apply an operation to a state 
-let do_s (s:concrete_st_s) (op:op_t) : concrete_st_s = 
+let do_s_direct (s:concrete_st_s_direct) (op:op_t) : concrete_st_s_direct = 
   do s op
 
 //equivalence relation between the concrete states of sequential type and MRDT
-let eq_sm (st_s:concrete_st_s) (st:concrete_st) = st_s == st
+let eq_sm_direct (st_s:concrete_st_s_direct) (st:concrete_st) = st_s == st
 
 //initial states are equivalent
-let initial_eq _
-  : Lemma (ensures eq_sm init_st_s init_st) = ()
+let initial_eq_direct _
+  : Lemma (ensures eq_sm_direct init_st_s_direct init_st) = ()
 
 //equivalence between states of sequential type and MRDT at every operation
-let do_eq (st_s:concrete_st_s) (st:concrete_st) (op:op_t)
-  : Lemma (requires eq_sm st_s st)
-          (ensures eq_sm (do_s st_s op) (do st op)) 
-  = do_prop st op
+let do_eq_direct (st_s:concrete_st_s_direct) (st:concrete_st) (op:op_t)
+  : Lemma (requires eq_sm_direct st_s st)
+          (ensures eq_sm_direct (do_s_direct st_s op) (do st op)) = ()
+  
+////////////////////////////////////////////////////////////////
+//// Linearization properties //////
+
+let merge1 (lca s1 s2:concrete_st)  =
+  let keys = S.union (M.domain lca) (S.union (M.domain s1) (M.domain s2)) in
+  let u:concrete_st = M.const_on keys S.empty in
+  M.iter_upd (fun k v -> S.union (sel lca k) (S.union (sel s1 k) (sel s2 k))) u
+
+let conv_prop1 (s:concrete_st) (op1 op2:op_t)
+  : Lemma (eq (do (do s op1) op2) (do (do s op2) op1)) = ()
+
+let conv_prop2 (lca s1 s2:concrete_st) (op:op_t) 
+  : Lemma (eq (do (merge1 lca s1 s2) op) (merge1 lca (do s1 op) s2)) = ()
+
+let conv_prop3 (lca s1 s2:concrete_st) (op:op_t) 
+  :  Lemma (eq (do (merge1 lca s1 s2) op) (merge1 lca s1 (do s2 op))) = 
+  conv_prop2 lca s2 s1 op
+
+let conv_prop4 (s:concrete_st)
+  : Lemma (eq (merge1 s s s) s) = ()
+
+let conv_prop5 (lca s1 s2:concrete_st) (op:op_t)
+  : Lemma (ensures eq (merge1 lca (do s1 op) (do s2 op)) (do (do (merge1 lca s1 s2) op) op)) = ()
   
 ////////////////////////////////////////////////////////////////
 
-let convergence1 (lca s1' s2:st) (o:op_t)
+////////////////////////////////////////////////////////////////
+//// Linearization properties - intermediate merge //////
+
+#push-options "--z3rlimit 100"
+let prop1 (l:concrete_st) (o1 o2 o3:op_t)
+  : Lemma (ensures eq (merge1 (do l o1) (do (do l o1) o2) (do (do l o3) o1)) (do (do (do l o3) o1) o2)) = ()
+
+let prop2 (l s s':concrete_st) (o1 o2 o3:op_t)
+  : Lemma (requires eq (merge1 s (do s o2) s') (do s' o2) /\
+                    eq (merge1 l s (do l o3)) s')
+          (ensures eq (merge1 (do s o1) (do (do s o1) o2) (do s' o1)) (do (do s' o1) o2)) = ()
+
+let prop3 (s s':concrete_st)
+  : Lemma (requires eq (merge1 s s s') s' /\
+                    (forall o2'. eq (merge1 s (do s o2') s') (do s' o2')))
+          (ensures (forall o2 o2'. (fst o2 <> fst o2') ==> eq (merge1 s (do (do s o2') o2) s') (do (do s' o2') o2))) = ()
+
+let lem_merge3 (l a b c:concrete_st) (op op':op_t) //cond3
+  : Lemma 
+    (requires eq (merge1 l a b) c /\ 
+              (forall (o:op_t). eq (merge1 l a (do b o)) (do c o)))
+    (ensures eq (merge1 l a (do (do b op) op')) (do (do c op) op')) = ()
+
+let prop4 (l s:concrete_st) (o1 o2 o3 o3':op_t)
+  : Lemma (requires (exists a b. eq (merge1 l a b) s) /\ //extra
+                    eq (merge1 (do l o1) (do (do l o1) o2) (do (do s o3) o1)) (do (do (do s o3) o1) o2))
+          (ensures eq (merge1 (do l o1) (do (do l o1) o2) (do (do (do s o3') o3) o1)) 
+                   (do (do (do (do s o3') o3) o1) o2)) = ()
+
+let lem_merge4 (s s':concrete_st) (op op':op_t) //cond4
+  : Lemma (requires eq (merge1 (do s op) (do s' op) (do s op)) (do s' op))
+          (ensures eq (merge1 (do s op) (do (do s' op') op) (do s op)) (do (do s' op') op)) = () 
+
+let idempotence (s:concrete_st) //automatic
+  : Lemma (eq (merge1 s s s) s) = ()
+
+let prop5' (l s s':concrete_st) (o o3:op_t)
+  : Lemma (requires eq (merge1 s s s') s' /\
+                    eq (merge1 l s (do l o3)) s')
+          (ensures eq (merge1 s s (do s' o)) (do s' o)) = ()
+          
+let prop5 (s s':concrete_st)
+  : Lemma (requires (exists a b. eq (merge1 s a b) s')) //extra
+          (ensures eq (merge1 s s s') s' /\ 
+                   eq (merge1 s s' s) s') = ()
+          
+////////////////////////////////////////////////////////////////
+
+(*let convergence1 (lca s1' s2:st) (o:op_t)
   : Lemma (requires //consistent_branches lca s1 s2 /\
                     //consistent_branches lca s1' s2 /\
                     (exists l1 l2 l3. apply_log (v_of lca) l1 == v_of s1' /\ apply_log (v_of lca) l2 == v_of s2 /\
@@ -289,4 +214,4 @@ let convergence2 (lca' lca s3 s1' s2:st)
           (ensures eq (concrete_merge (v_of lca') (concrete_merge (v_of lca) (v_of s3) (v_of s1')) (v_of s2)) 
                       (concrete_merge (v_of s1') 
                                        (concrete_merge (v_of lca) (v_of s3) (v_of s1'))
-                                       (concrete_merge (v_of lca') (v_of s1') (v_of s2)))) = ()
+                                       (concrete_merge (v_of lca') (v_of s1') (v_of s2)))) = ()*)
